-

dp/6_1.dfy
@@ -19,8 +19,28 @@ module SixOne {
     {
         if |a| == 0 then [] else
         if |a| == 1 then [a[0]] else 
-        if a2([a[0]], a2(a, a1(a[1..])))==[a[0]] then [a[0]]
-        else if a2(a, a1(a[1..])) == a then a else a1(a[1..])
+        if a2([a[0]], a2(a, a1(a[1..])))==[a[0]] then [a[0]] else
+        if a2(a, a1(a[1..])) == a then a else a1(a[1..])
+    }
+
+    function a1'(a: seq<int>, i: nat): seq<int>
+    decreases i
+    requires 0<=i<|a|
+    {
+        if |a|==0 then [] else
+        if i==0 then [a[i]] else 
+        if a2([], a1'(a,i-1)+[a[i]]) == [] then [] else
+        a1'(a,i-1)+[a[i]] 
+    }
+
+    function a1''(a: seq<int>, i: nat): int
+    decreases i
+    requires 0<=i<|a|
+    {
+        if |a|==0 then 0 else
+        if i==0 then a[i] else 
+        if a2([], a1'(a,i-1)+[a[i]]) == [] then 0 else
+        S.seqSum(a1'(a,i-1))+a[i]
     }
 
     function a2(a: seq<int>, b: seq<int>): seq<int>
@@ -32,26 +52,39 @@ module SixOne {
         if M.max(S.seqSum(a), S.seqSum(b)) == S.seqSum(a) then a else b
     }
 
-    /**
-     * Axiom 1': Express Axiom 1
-     * in inductive form for Dafny, if needed.
-     */
-
     method Main()
     {
         // Base case.
         var a := [0];
         assert a1(a) == a;
+        assert a1'(a, |a|-1) == a;
 
-        /*
-        var a'', a''' := [1, 0], [0, 0];
-        assert a2(a'', a''') == a'';
-        */
+        var e := [0, 1];
+        assert a1''(e, |e|-1) == 1;
+        assert a1'(e, |e|-1) == e;
+        assert a1(e) == e;
 
         var a' := [1, 0];
-        assert a1(a') == a';
+        assert a1'(a', |a'|-1) == a';
+        assert a1(a) == a';
+
+        var c' := [-1, 1];
+        var c'_ans := [1];
+        assert a1(c') == c'_ans;
+        assert a1'(c', |c'|-1) == c'_ans;
+
+        var c := [-1, 1, 2];
+        var c_ans := [1, 2];
+        assert a1(c) == c_ans;
+        assert a1'(c, |c|-1) == c_ans;
+
+        var d := [-1, 1, 2, -2];
+        var d_ans := [1, 2];
+        assert a1(d) == d_ans;
+
 
         var b := [5,15,-30,10,-5,40,10];
-        assert a1(b) == [10,-5,40,10];
+        var b_ans := [10,-5,40,10];
+        assert a1(b) == b_ans;
     }
 }
